theories/examples.v
@@ -3,25 +3,26 @@ From stbor Require Import notation tactics.
 (** Some common types *)
 Notation int := (Scala 1).
 Notation int_arr n := (Scala n).
-Notation "'!&mut' T" := (Reference (RefPtr Mutable) T) (at level 10, format "!&mut  T").
-Notation "'!&' T" := (Reference (RefPtr Immutable) T) (at level 10, format "!&  T").
-Notation "'!*' T" := (Reference RawPtr T) (at level 10, format "!*  T").
+Notation "'ᵗ&mut' T" := (Reference (RefPtr Mutable) T) (at level 10, format "ᵗ&mut  T").
+Notation "'ᵗ&' T" := (Reference (RefPtr Immutable) T) (at level 10, format "ᵗ&  T").
+Notation "'ᵗ*' T" := (Reference RawPtr T) (at level 10, format "ᵗ*  T").
 Notation "'Box<' T '>'" := (Reference RawPtr T) (at level 10, format "Box< T >").
 
 
-Notation "@& e" := (Ref e%E) (at level 9, format "@& e") : expr_scope.
-Notation "'@*' T '/' N e" := (Deref e%E T N) (at level 8, format "@* T / N  e") : expr_scope.
+Notation "ᵛ& e" := (Ref e%E) (at level 9, format "ᵛ& e") : expr_scope.
+Notation "ᵛ*{ T , N } e" := (Deref e%E T N) (at level 8, format "ᵛ*{ T ,  N }  e") : expr_scope.
 
 Definition new_zero amod : val :=
-  λ: [<>], let: "i" := Alloc int amod in "i" <- #0 ;; @&"i".
+  λ: [<>], let: "i" := Alloc int amod in "i" <- #0 ;; ᵛ&"i".
 Definition new_mut_ref_int amod : val :=
   λ: ["v"],
-    let: "x" := Alloc (!&mut int) amod in
+    let: "x" := Alloc (ᵗ&mut int) amod in
       "x" <- "v" ;; "x".
 
 Definition demo0 : val :=
   λ: ["x"],
-  let: "y" := new_mut_ref_int Stack [  @& (Deref (!"x") int (Some Mutable) ) ] in
-  (Deref (!"y") int (Some Mutable) ) <- #5 ;;
-  (Deref (!"x") int (Some Mutable) ) <- #5 ;;
-  !(Deref (!"y") int (Some Mutable) ).
+  let: "y" := new_mut_ref_int Stack [ ᵛ& ᵛ*{int, Some Mutable} (!"x") ] in
+  Retag "y" (ᵗ&mut int) Default ;;
+  ᵛ*{int, Some Mutable} (!"y") <- #5 ;;
+  ᵛ*{int, Some Mutable} (!"x") <- #3 ;;
+  !(ᵛ*{int, Some Mutable} (!"y")).
